<?xml version="1.0"?>
<rdf:RDF xmlns="http://www.semanticweb.org/allalihoussam/ontologies/2025/3/untitled-ontology-11/"
     xml:base="http://www.semanticweb.org/allalihoussam/ontologies/2025/3/untitled-ontology-11/"
     xmlns:owl="http://www.w3.org/2002/07/owl#"
     xmlns:rdf="http://www.w3.org/1999/02/22-rdf-syntax-ns#"
     xmlns:xml="http://www.w3.org/XML/1998/namespace"
     xmlns:xsd="http://www.w3.org/2001/XMLSchema#"
     xmlns:rdfs="http://www.w3.org/2000/01/rdf-schema#"
     xmlns:terms="http://purl.org/dc/terms/">
    <owl:Ontology rdf:about="http://example.com/TripPlanningOntology">
        <terms:creator>Houssam Allali</terms:creator>
        <rdfs:label>Trip Planning Ontology</rdfs:label>
        <owl:versionInfo>v1.0</owl:versionInfo>
    </owl:Ontology>
    


    <!-- 
    ///////////////////////////////////////////////////////////////////////////////////////
    //
    // Annotation properties
    //
    ///////////////////////////////////////////////////////////////////////////////////////
     -->

    


    <!-- http://purl.org/dc/terms/creator -->

    <owl:AnnotationProperty rdf:about="http://purl.org/dc/terms/creator"/>
    


    <!-- 
    ///////////////////////////////////////////////////////////////////////////////////////
    //
    // Object Properties
    //
    ///////////////////////////////////////////////////////////////////////////////////////
     -->

    


    <!-- http://example.com/TripPlanningOntology#hasWeather -->

    <owl:ObjectProperty rdf:about="http://example.com/TripPlanningOntology#hasWeather">
        <owl:inverseOf rdf:resource="http://example.com/TripPlanningOntology#isWeatherFor"/>
        <rdfs:domain rdf:resource="http://www.semanticweb.org/allalihoussam/ontologies/2025/3/untitled-ontology-11/TripSegment"/>
        <rdfs:range rdf:resource="http://example.com/TripPlanningOntology#Weather"/>
    </owl:ObjectProperty>
    


    <!-- http://example.com/TripPlanningOntology#isWeatherFor -->

    <owl:ObjectProperty rdf:about="http://example.com/TripPlanningOntology#isWeatherFor"/>
    


    <!-- http://www.semanticweb.org/allalihoussam/ontologies/2025/3/untitled-ontology-11/hasAffordance -->

    <owl:ObjectProperty rdf:about="http://www.semanticweb.org/allalihoussam/ontologies/2025/3/untitled-ontology-11/hasAffordance">
        <rdfs:domain rdf:resource="http://www.semanticweb.org/allalihoussam/ontologies/2025/3/untitled-ontology-11/Operation"/>
        <rdfs:comment>“Points to a Web of Things affordance describing how an operation can be invoked (e.g., REST endpoint, MQTT topic, etc.).”</rdfs:comment>
    </owl:ObjectProperty>
    


    <!-- http://www.semanticweb.org/allalihoussam/ontologies/2025/3/untitled-ontology-11/hasConnection -->

    <owl:ObjectProperty rdf:about="http://www.semanticweb.org/allalihoussam/ontologies/2025/3/untitled-ontology-11/hasConnection">
        <rdfs:domain rdf:resource="http://www.semanticweb.org/allalihoussam/ontologies/2025/3/untitled-ontology-11/TripSegment"/>
        <rdfs:range rdf:resource="http://www.semanticweb.org/allalihoussam/ontologies/2025/3/untitled-ontology-11/Connection"/>
        <rdfs:comment>“Indicates that a trip segment involves at least one Connection, requiring passengers to change vehicles or carriers.”</rdfs:comment>
        <rdfs:label>has connection</rdfs:label>
    </owl:ObjectProperty>
    


    <!-- http://www.semanticweb.org/allalihoussam/ontologies/2025/3/untitled-ontology-11/hasItinerary -->

    <owl:ObjectProperty rdf:about="http://www.semanticweb.org/allalihoussam/ontologies/2025/3/untitled-ontology-11/hasItinerary">
        <rdfs:domain rdf:resource="http://www.semanticweb.org/allalihoussam/ontologies/2025/3/untitled-ontology-11/TripPlan"/>
        <rdfs:range rdf:resource="http://www.semanticweb.org/allalihoussam/ontologies/2025/3/untitled-ontology-11/Itinerary"/>
        <rdfs:comment>“Links a Trip Plan to one or more Itinerary objects (Trip Segments). An itinerary can contain departure and arrival times, modes, and connections.”</rdfs:comment>
        <rdfs:label>has itinerary</rdfs:label>
    </owl:ObjectProperty>
    


    <!-- http://www.semanticweb.org/allalihoussam/ontologies/2025/3/untitled-ontology-11/hasMode -->

    <owl:ObjectProperty rdf:about="http://www.semanticweb.org/allalihoussam/ontologies/2025/3/untitled-ontology-11/hasMode">
        <rdfs:domain rdf:resource="http://www.semanticweb.org/allalihoussam/ontologies/2025/3/untitled-ontology-11/TripSegment"/>
        <rdfs:range rdf:resource="http://www.semanticweb.org/allalihoussam/ontologies/2025/3/untitled-ontology-11/TransportationMode"/>
        <rdfs:comment>“States which Transportation Mode (train, bus, plane, etc.) is used for this Trip Segment.”</rdfs:comment>
        <rdfs:label>has mode</rdfs:label>
    </owl:ObjectProperty>
    


    <!-- http://www.semanticweb.org/allalihoussam/ontologies/2025/3/untitled-ontology-11/hasOperation -->

    <owl:ObjectProperty rdf:about="http://www.semanticweb.org/allalihoussam/ontologies/2025/3/untitled-ontology-11/hasOperation">
        <rdfs:domain rdf:resource="http://www.semanticweb.org/allalihoussam/ontologies/2025/3/untitled-ontology-11/TripPlanningService"/>
        <rdfs:range rdf:resource="http://www.semanticweb.org/allalihoussam/ontologies/2025/3/untitled-ontology-11/Operation"/>
        <rdfs:comment>“Associates a Trip Planning Service with the operations it provides (e.g., planning, booking, schedule lookup).”</rdfs:comment>
        <rdfs:label>has operation</rdfs:label>
    </owl:ObjectProperty>
    


    <!-- http://www.semanticweb.org/allalihoussam/ontologies/2025/3/untitled-ontology-11/hasPricingModel -->

    <owl:ObjectProperty rdf:about="http://www.semanticweb.org/allalihoussam/ontologies/2025/3/untitled-ontology-11/hasPricingModel">
        <rdfs:domain rdf:resource="http://www.semanticweb.org/allalihoussam/ontologies/2025/3/untitled-ontology-11/TripSegment"/>
        <rdfs:range rdf:resource="http://www.semanticweb.org/allalihoussam/ontologies/2025/3/untitled-ontology-11/PricingModel"/>
        <rdfs:comment>“Identifies which Pricing Model (fixed or dynamic) applies to this Trip Segment. Useful for cost calculation or agent’s reasoning about fare changes.”</rdfs:comment>
        <rdfs:label>has pricing model</rdfs:label>
    </owl:ObjectProperty>
    


    <!-- http://www.semanticweb.org/allalihoussam/ontologies/2025/3/untitled-ontology-11/hasReturnTrip -->

    <owl:ObjectProperty rdf:about="http://www.semanticweb.org/allalihoussam/ontologies/2025/3/untitled-ontology-11/hasReturnTrip">
        <rdf:type rdf:resource="http://www.w3.org/2002/07/owl#InverseFunctionalProperty"/>
        <rdfs:domain rdf:resource="http://www.semanticweb.org/allalihoussam/ontologies/2025/3/untitled-ontology-11/RoundTripPlan"/>
        <rdfs:range rdf:resource="http://www.semanticweb.org/allalihoussam/ontologies/2025/3/untitled-ontology-11/TripSegment"/>
        <rdfs:comment>“Connects a round trip plan to its return trip segment, if any. Generally used when modeling a round journey with outbound and return details.”</rdfs:comment>
        <rdfs:label>has return trip</rdfs:label>
    </owl:ObjectProperty>
    


    <!-- http://www.semanticweb.org/allalihoussam/ontologies/2025/3/untitled-ontology-11/hasStop -->

    <owl:ObjectProperty rdf:about="http://www.semanticweb.org/allalihoussam/ontologies/2025/3/untitled-ontology-11/hasStop">
        <rdfs:domain rdf:resource="http://www.semanticweb.org/allalihoussam/ontologies/2025/3/untitled-ontology-11/TransportationLine"/>
        <rdfs:range rdf:resource="http://www.semanticweb.org/allalihoussam/ontologies/2025/3/untitled-ontology-11/Stop"/>
        <rdfs:comment>“Indicates all the stops serviced by a particular Transportation Line, in order or not. Each stop is a distinct location.”</rdfs:comment>
        <rdfs:label>has stop</rdfs:label>
    </owl:ObjectProperty>
    


    <!-- http://www.semanticweb.org/allalihoussam/ontologies/2025/3/untitled-ontology-11/usesTransportationLine -->

    <owl:ObjectProperty rdf:about="http://www.semanticweb.org/allalihoussam/ontologies/2025/3/untitled-ontology-11/usesTransportationLine">
        <rdfs:domain rdf:resource="http://www.semanticweb.org/allalihoussam/ontologies/2025/3/untitled-ontology-11/TripSegment"/>
        <rdfs:range rdf:resource="http://www.semanticweb.org/allalihoussam/ontologies/2025/3/untitled-ontology-11/TransportationLine"/>
        <rdfs:comment>“Specifies which Transportation Line is used for a given Trip Segment (e.g., which train or bus line a traveler rides).”</rdfs:comment>
        <rdfs:label>uses transportation line</rdfs:label>
    </owl:ObjectProperty>
    


    <!-- 
    ///////////////////////////////////////////////////////////////////////////////////////
    //
    // Data properties
    //
    ///////////////////////////////////////////////////////////////////////////////////////
     -->

    


    <!-- http://example.com/TripPlanningOntology#conditions -->

    <owl:DatatypeProperty rdf:about="http://example.com/TripPlanningOntology#conditions">
        <rdfs:domain rdf:resource="http://example.com/TripPlanningOntology#Weather"/>
        <rdfs:range rdf:resource="http://www.w3.org/2001/XMLSchema#string"/>
    </owl:DatatypeProperty>
    


    <!-- http://example.com/TripPlanningOntology#forecastDate -->

    <owl:DatatypeProperty rdf:about="http://example.com/TripPlanningOntology#forecastDate">
        <rdfs:domain rdf:resource="http://example.com/TripPlanningOntology#Weather"/>
        <rdfs:range rdf:resource="http://www.w3.org/2001/XMLSchema#dateTime"/>
    </owl:DatatypeProperty>
    


    <!-- http://example.com/TripPlanningOntology#pricePerNight -->

    <owl:DatatypeProperty rdf:about="http://example.com/TripPlanningOntology#pricePerNight">
        <rdfs:domain rdf:resource="http://example.com/TripPlanningOntology#Accommodation"/>
        <rdfs:range rdf:resource="http://www.w3.org/2001/XMLSchema#decimal"/>
    </owl:DatatypeProperty>
    


    <!-- http://example.com/TripPlanningOntology#temperature -->

    <owl:DatatypeProperty rdf:about="http://example.com/TripPlanningOntology#temperature">
        <rdfs:domain rdf:resource="http://example.com/TripPlanningOntology#Weather"/>
        <rdfs:range rdf:resource="http://www.w3.org/2001/XMLSchema#float"/>
        <rdfs:label>The avergae temprature of the eather during the trip.</rdfs:label>
    </owl:DatatypeProperty>
    


    <!-- http://example.com/TripPlanningOntology#windSpeed -->

    <owl:DatatypeProperty rdf:about="http://example.com/TripPlanningOntology#windSpeed">
        <rdfs:domain rdf:resource="http://example.com/TripPlanningOntology#Weather"/>
        <rdfs:range rdf:resource="http://www.w3.org/2001/XMLSchema#float"/>
    </owl:DatatypeProperty>
    


    <!-- http://www.semanticweb.org/allalihoussam/ontologies/2025/3/untitled-ontology-11/arrivalInput -->

    <owl:DatatypeProperty rdf:about="http://www.semanticweb.org/allalihoussam/ontologies/2025/3/untitled-ontology-11/arrivalInput">
        <rdfs:domain rdf:resource="http://www.semanticweb.org/allalihoussam/ontologies/2025/3/untitled-ontology-11/TripPlan"/>
        <rdfs:range rdf:resource="http://www.w3.org/2001/XMLSchema#string"/>
        <rdfs:comment>“The user’s textual input indicating the destination location for the trip plan (e.g., ‘London’).”</rdfs:comment>
        <rdfs:label>arrival input</rdfs:label>
    </owl:DatatypeProperty>
    


    <!-- http://www.semanticweb.org/allalihoussam/ontologies/2025/3/untitled-ontology-11/departureDateInput -->

    <owl:DatatypeProperty rdf:about="http://www.semanticweb.org/allalihoussam/ontologies/2025/3/untitled-ontology-11/departureDateInput">
        <rdfs:domain rdf:resource="http://www.semanticweb.org/allalihoussam/ontologies/2025/3/untitled-ontology-11/TripPlan"/>
        <rdfs:range rdf:resource="http://www.w3.org/2001/XMLSchema#dateTime"/>
        <rdfs:comment>“Specifies the planned departure date and time (in ISO dateTime format) for the forward journey.”</rdfs:comment>
        <rdfs:label>departure date input</rdfs:label>
    </owl:DatatypeProperty>
    


    <!-- http://www.semanticweb.org/allalihoussam/ontologies/2025/3/untitled-ontology-11/departureInput -->

    <owl:DatatypeProperty rdf:about="http://www.semanticweb.org/allalihoussam/ontologies/2025/3/untitled-ontology-11/departureInput">
        <rdfs:domain rdf:resource="http://www.semanticweb.org/allalihoussam/ontologies/2025/3/untitled-ontology-11/TripPlan"/>
        <rdfs:range rdf:resource="http://www.w3.org/2001/XMLSchema#string"/>
        <rdfs:comment>“The user’s (or agent’s) textual input representing the origin location (e.g., ‘Paris’). Could be a city name, station code, or geolocation.”</rdfs:comment>
        <rdfs:label>departure input</rdfs:label>
    </owl:DatatypeProperty>
    


    <!-- http://www.semanticweb.org/allalihoussam/ontologies/2025/3/untitled-ontology-11/duration -->

    <owl:DatatypeProperty rdf:about="http://www.semanticweb.org/allalihoussam/ontologies/2025/3/untitled-ontology-11/duration">
        <rdfs:domain rdf:resource="http://www.semanticweb.org/allalihoussam/ontologies/2025/3/untitled-ontology-11/TripSegment"/>
        <rdfs:range rdf:resource="http://www.w3.org/2001/XMLSchema#integer"/>
        <rdfs:comment>“Total travel time for the segment, typically expressed in minutes.”</rdfs:comment>
        <rdfs:label>duration</rdfs:label>
    </owl:DatatypeProperty>
    


    <!-- http://www.semanticweb.org/allalihoussam/ontologies/2025/3/untitled-ontology-11/isInternational -->

    <owl:DatatypeProperty rdf:about="http://www.semanticweb.org/allalihoussam/ontologies/2025/3/untitled-ontology-11/isInternational">
        <rdfs:range rdf:resource="http://www.w3.org/2001/XMLSchema#boolean"/>
        <rdfs:label>is international</rdfs:label>
    </owl:DatatypeProperty>
    


    <!-- http://www.semanticweb.org/allalihoussam/ontologies/2025/3/untitled-ontology-11/maxConnectionsAllowed -->

    <owl:DatatypeProperty rdf:about="http://www.semanticweb.org/allalihoussam/ontologies/2025/3/untitled-ontology-11/maxConnectionsAllowed">
        <rdfs:domain rdf:resource="http://www.semanticweb.org/allalihoussam/ontologies/2025/3/untitled-ontology-11/PlanTripOperation"/>
        <rdfs:range rdf:resource="http://www.w3.org/2001/XMLSchema#integer"/>
        <rdfs:comment>“Specifies the maximum number of transfers/connections permitted when planning an itinerary. Useful for limiting overly complex multi‐leg trips.”</rdfs:comment>
        <rdfs:label>max connections allowed</rdfs:label>
    </owl:DatatypeProperty>
    


    <!-- http://www.semanticweb.org/allalihoussam/ontologies/2025/3/untitled-ontology-11/modeName -->

    <owl:DatatypeProperty rdf:about="http://www.semanticweb.org/allalihoussam/ontologies/2025/3/untitled-ontology-11/modeName">
        <rdfs:domain rdf:resource="http://www.semanticweb.org/allalihoussam/ontologies/2025/3/untitled-ontology-11/TransportationMode"/>
        <rdfs:range rdf:resource="http://www.w3.org/2001/XMLSchema#string"/>
        <rdfs:comment>“Human‐readable name of the transportation mode (e.g. ‘Train’, ‘Bus’, ‘Airplane’), to be displayed in user interfaces.”</rdfs:comment>
        <rdfs:label>mode name</rdfs:label>
    </owl:DatatypeProperty>
    


    <!-- http://www.semanticweb.org/allalihoussam/ontologies/2025/3/untitled-ontology-11/price -->

    <owl:DatatypeProperty rdf:about="http://www.semanticweb.org/allalihoussam/ontologies/2025/3/untitled-ontology-11/price">
        <rdfs:domain rdf:resource="http://www.semanticweb.org/allalihoussam/ontologies/2025/3/untitled-ontology-11/TripSegment"/>
        <rdfs:range rdf:resource="http://www.w3.org/2001/XMLSchema#decimal"/>
        <rdfs:comment>“Represents the base fare or cost (as a decimal number) for a single Trip Segment. Usually expressed in a specific currency.”</rdfs:comment>
        <rdfs:label>price</rdfs:label>
    </owl:DatatypeProperty>
    


    <!-- http://www.semanticweb.org/allalihoussam/ontologies/2025/3/untitled-ontology-11/priceCurrency -->

    <owl:DatatypeProperty rdf:about="http://www.semanticweb.org/allalihoussam/ontologies/2025/3/untitled-ontology-11/priceCurrency">
        <rdfs:domain rdf:resource="http://www.semanticweb.org/allalihoussam/ontologies/2025/3/untitled-ontology-11/TripSegment"/>
        <rdfs:range rdf:resource="http://www.w3.org/2001/XMLSchema#string"/>
        <rdfs:comment>“ISO currency code or textual label (e.g., ‘USD’, ‘EUR’) specifying the currency for the ‘price’ value of this segment.”</rdfs:comment>
        <rdfs:label>price currency</rdfs:label>
    </owl:DatatypeProperty>
    


    <!-- http://www.semanticweb.org/allalihoussam/ontologies/2025/3/untitled-ontology-11/remainingSeats -->

    <owl:DatatypeProperty rdf:about="http://www.semanticweb.org/allalihoussam/ontologies/2025/3/untitled-ontology-11/remainingSeats">
        <rdfs:domain rdf:resource="http://www.semanticweb.org/allalihoussam/ontologies/2025/3/untitled-ontology-11/TripSegment"/>
        <rdfs:range rdf:resource="http://www.w3.org/2001/XMLSchema#integer"/>
        <rdfs:comment>“Number of seats still available for booking on this segment. Can help an agent decide whether to show an alert for limited availability.”</rdfs:comment>
        <rdfs:label>remaining seats</rdfs:label>
    </owl:DatatypeProperty>
    


    <!-- http://www.semanticweb.org/allalihoussam/ontologies/2025/3/untitled-ontology-11/returnDateInput -->

    <owl:DatatypeProperty rdf:about="http://www.semanticweb.org/allalihoussam/ontologies/2025/3/untitled-ontology-11/returnDateInput">
        <rdfs:domain rdf:resource="http://www.semanticweb.org/allalihoussam/ontologies/2025/3/untitled-ontology-11/TripPlan"/>
        <rdfs:range rdf:resource="http://www.w3.org/2001/XMLSchema#dateTime"/>
        <rdfs:comment>“Specifies the planned departure date and time for the return journey (if applicable). Relevant primarily in round trip contexts.”</rdfs:comment>
        <rdfs:label>return date input</rdfs:label>
    </owl:DatatypeProperty>
    


    <!-- http://www.semanticweb.org/allalihoussam/ontologies/2025/3/untitled-ontology-11/transferTime -->

    <owl:DatatypeProperty rdf:about="http://www.semanticweb.org/allalihoussam/ontologies/2025/3/untitled-ontology-11/transferTime">
        <rdfs:domain rdf:resource="http://www.semanticweb.org/allalihoussam/ontologies/2025/3/untitled-ontology-11/Connection"/>
        <rdfs:range rdf:resource="http://www.w3.org/2001/XMLSchema#integer"/>
        <rdfs:comment>“Time available/required for passengers to switch from one vehicle to another. Important in multi‐segment journeys.”</rdfs:comment>
        <rdfs:label>transfer time</rdfs:label>
    </owl:DatatypeProperty>
    


    <!-- 
    ///////////////////////////////////////////////////////////////////////////////////////
    //
    // Classes
    //
    ///////////////////////////////////////////////////////////////////////////////////////
     -->

    


    <!-- http://example.com/TripPlanningOntology#Accommodation -->

    <owl:Class rdf:about="http://example.com/TripPlanningOntology#Accommodation"/>
    


    <!-- http://example.com/TripPlanningOntology#Hostel -->

    <owl:Class rdf:about="http://example.com/TripPlanningOntology#Hostel">
        <rdfs:subClassOf rdf:resource="http://example.com/TripPlanningOntology#Accommodation"/>
    </owl:Class>
    


    <!-- http://example.com/TripPlanningOntology#Hotel -->

    <owl:Class rdf:about="http://example.com/TripPlanningOntology#Hotel">
        <rdfs:subClassOf rdf:resource="http://example.com/TripPlanningOntology#Accommodation"/>
    </owl:Class>
    


    <!-- http://example.com/TripPlanningOntology#Rainy -->

    <owl:Class rdf:about="http://example.com/TripPlanningOntology#Rainy">
        <rdfs:subClassOf rdf:resource="http://example.com/TripPlanningOntology#Weather"/>
    </owl:Class>
    


    <!-- http://example.com/TripPlanningOntology#Snowy -->

    <owl:Class rdf:about="http://example.com/TripPlanningOntology#Snowy">
        <rdfs:subClassOf rdf:resource="http://example.com/TripPlanningOntology#Weather"/>
    </owl:Class>
    


    <!-- http://example.com/TripPlanningOntology#Sunny -->

    <owl:Class rdf:about="http://example.com/TripPlanningOntology#Sunny">
        <rdfs:subClassOf rdf:resource="http://example.com/TripPlanningOntology#Weather"/>
    </owl:Class>
    


    <!-- http://example.com/TripPlanningOntology#VacationRental -->

    <owl:Class rdf:about="http://example.com/TripPlanningOntology#VacationRental">
        <rdfs:subClassOf rdf:resource="http://example.com/TripPlanningOntology#Accommodation"/>
    </owl:Class>
    


    <!-- http://example.com/TripPlanningOntology#Weather -->

    <owl:Class rdf:about="http://example.com/TripPlanningOntology#Weather"/>
    


    <!-- http://www.semanticweb.org/allalihoussam/ontologies/2025/3/untitled-ontology-11/Connection -->

    <owl:Class rdf:about="http://www.semanticweb.org/allalihoussam/ontologies/2025/3/untitled-ontology-11/Connection">
        <rdfs:subClassOf>
            <owl:Restriction>
                <owl:onProperty rdf:resource="http://www.semanticweb.org/allalihoussam/ontologies/2025/3/untitled-ontology-11/transferTime"/>
                <owl:qualifiedCardinality rdf:datatype="http://www.w3.org/2001/XMLSchema#nonNegativeInteger">1</owl:qualifiedCardinality>
                <owl:onDataRange rdf:resource="http://www.w3.org/2001/XMLSchema#integer"/>
            </owl:Restriction>
        </rdfs:subClassOf>
        <rdfs:comment>“A scheduled link between two trip segments where the passenger changes vehicles (or carriers). May involve transfer time, possibly in a station or hub.”</rdfs:comment>
        <rdfs:label>Connection</rdfs:label>
    </owl:Class>
    


    <!-- http://www.semanticweb.org/allalihoussam/ontologies/2025/3/untitled-ontology-11/DynamicPricingModel -->

    <owl:Class rdf:about="http://www.semanticweb.org/allalihoussam/ontologies/2025/3/untitled-ontology-11/DynamicPricingModel">
        <rdfs:subClassOf rdf:resource="http://www.semanticweb.org/allalihoussam/ontologies/2025/3/untitled-ontology-11/PricingModel"/>
        <owl:disjointWith rdf:resource="http://www.semanticweb.org/allalihoussam/ontologies/2025/3/untitled-ontology-11/FixedPricingModel"/>
        <rdfs:comment>“A pricing approach where the cost can fluctuate based on remaining seats, demand, or other real-time factors.”</rdfs:comment>
        <rdfs:label>Dynamic Pricing Model</rdfs:label>
    </owl:Class>
    


    <!-- http://www.semanticweb.org/allalihoussam/ontologies/2025/3/untitled-ontology-11/FixedPricingModel -->

    <owl:Class rdf:about="http://www.semanticweb.org/allalihoussam/ontologies/2025/3/untitled-ontology-11/FixedPricingModel">
        <rdfs:subClassOf rdf:resource="http://www.semanticweb.org/allalihoussam/ontologies/2025/3/untitled-ontology-11/PricingModel"/>
        <rdfs:comment>“A pricing strategy where the fare remains constant regardless of timing, demand, or seat availability.”</rdfs:comment>
        <rdfs:label>Fixed Pricing Model</rdfs:label>
    </owl:Class>
    


    <!-- http://www.semanticweb.org/allalihoussam/ontologies/2025/3/untitled-ontology-11/InternationalTrip -->

    <owl:Class rdf:about="http://www.semanticweb.org/allalihoussam/ontologies/2025/3/untitled-ontology-11/InternationalTrip">
        <rdfs:subClassOf rdf:resource="http://www.semanticweb.org/allalihoussam/ontologies/2025/3/untitled-ontology-11/TripSegment"/>
        <rdfs:comment>“Denotes a trip segment that crosses at least one national border. Typically associated with additional constraints or documentation.”</rdfs:comment>
        <rdfs:label>International Trip</rdfs:label>
    </owl:Class>
    


    <!-- http://www.semanticweb.org/allalihoussam/ontologies/2025/3/untitled-ontology-11/Itinerary -->

    <owl:Class rdf:about="http://www.semanticweb.org/allalihoussam/ontologies/2025/3/untitled-ontology-11/Itinerary">
        <rdfs:comment>“Represents a structured travel plan detailing how to go from an origin to a destination, potentially including multiple modes of transport and segments.”</rdfs:comment>
        <rdfs:label>Itinerary</rdfs:label>
    </owl:Class>
    


    <!-- http://www.semanticweb.org/allalihoussam/ontologies/2025/3/untitled-ontology-11/OneWayTrip -->

    <owl:Class rdf:about="http://www.semanticweb.org/allalihoussam/ontologies/2025/3/untitled-ontology-11/OneWayTrip">
        <rdfs:subClassOf rdf:resource="http://www.semanticweb.org/allalihoussam/ontologies/2025/3/untitled-ontology-11/TripSegment"/>
        <rdfs:comment>“A trip segment with no return component, going from the departure point directly to the destination.”</rdfs:comment>
        <rdfs:label>One Way Trip</rdfs:label>
    </owl:Class>
    


    <!-- http://www.semanticweb.org/allalihoussam/ontologies/2025/3/untitled-ontology-11/Operation -->

    <owl:Class rdf:about="http://www.semanticweb.org/allalihoussam/ontologies/2025/3/untitled-ontology-11/Operation">
        <rdfs:comment>“A generic type of action that can be performed on a Trip Planning Service. Examples include trip planning requests, ticket booking, or retrieving schedule information.”</rdfs:comment>
        <rdfs:label>Operation</rdfs:label>
    </owl:Class>
    


    <!-- http://www.semanticweb.org/allalihoussam/ontologies/2025/3/untitled-ontology-11/PlanTripOperation -->

    <owl:Class rdf:about="http://www.semanticweb.org/allalihoussam/ontologies/2025/3/untitled-ontology-11/PlanTripOperation">
        <rdfs:subClassOf rdf:resource="http://www.semanticweb.org/allalihoussam/ontologies/2025/3/untitled-ontology-11/Operation"/>
        <rdfs:subClassOf>
            <owl:Restriction>
                <owl:onProperty rdf:resource="http://www.semanticweb.org/allalihoussam/ontologies/2025/3/untitled-ontology-11/maxConnectionsAllowed"/>
                <owl:qualifiedCardinality rdf:datatype="http://www.w3.org/2001/XMLSchema#nonNegativeInteger">1</owl:qualifiedCardinality>
                <owl:onDataRange rdf:resource="http://www.w3.org/2001/XMLSchema#integer"/>
            </owl:Restriction>
        </rdfs:subClassOf>
        <rdfs:comment>“A specialized operation that allows the user (or an agent) to request a trip plan based on input parameters, such as origin, destination, dates, and possibly other constraints (like max connections).”</rdfs:comment>
        <rdfs:label>Plan Trip Operation</rdfs:label>
    </owl:Class>
    


    <!-- http://www.semanticweb.org/allalihoussam/ontologies/2025/3/untitled-ontology-11/PricingModel -->

    <owl:Class rdf:about="http://www.semanticweb.org/allalihoussam/ontologies/2025/3/untitled-ontology-11/PricingModel">
        <rdfs:comment>“Describes how the fare or cost for a trip (or trip segment) is determined. Could be fixed or variable depending on certain factors like seat availability.”</rdfs:comment>
        <rdfs:label>Pricing Model</rdfs:label>
    </owl:Class>
    


    <!-- http://www.semanticweb.org/allalihoussam/ontologies/2025/3/untitled-ontology-11/RoundTripPlan -->

    <owl:Class rdf:about="http://www.semanticweb.org/allalihoussam/ontologies/2025/3/untitled-ontology-11/RoundTripPlan">
        <rdfs:subClassOf rdf:resource="http://www.semanticweb.org/allalihoussam/ontologies/2025/3/untitled-ontology-11/TripPlan"/>
        <rdfs:comment>“A specialized trip plan containing at least one forward trip segment and a corresponding return trip. Often includes separate outbound and return dates.”</rdfs:comment>
        <rdfs:label>Round Trip Plan</rdfs:label>
    </owl:Class>
    


    <!-- http://www.semanticweb.org/allalihoussam/ontologies/2025/3/untitled-ontology-11/Stop -->

    <owl:Class rdf:about="http://www.semanticweb.org/allalihoussam/ontologies/2025/3/untitled-ontology-11/Stop">
        <rdfs:comment>“A station or stop along a transportation line where passengers can board or alight. May be a bus stop, train station, airport terminal, etc.”</rdfs:comment>
        <rdfs:label>Stop</rdfs:label>
    </owl:Class>
    


    <!-- http://www.semanticweb.org/allalihoussam/ontologies/2025/3/untitled-ontology-11/TransportationLine -->

    <owl:Class rdf:about="http://www.semanticweb.org/allalihoussam/ontologies/2025/3/untitled-ontology-11/TransportationLine">
        <rdfs:subClassOf>
            <owl:Restriction>
                <owl:onProperty rdf:resource="http://www.semanticweb.org/allalihoussam/ontologies/2025/3/untitled-ontology-11/hasStop"/>
                <owl:minQualifiedCardinality rdf:datatype="http://www.w3.org/2001/XMLSchema#nonNegativeInteger">1</owl:minQualifiedCardinality>
                <owl:onClass rdf:resource="http://www.semanticweb.org/allalihoussam/ontologies/2025/3/untitled-ontology-11/Stop"/>
            </owl:Restriction>
        </rdfs:subClassOf>
        <rdfs:comment>“A named or coded line (e.g., a bus line or train line) that services specific stops. Multiple segments can use the same line.”</rdfs:comment>
        <rdfs:label>Transportation Line</rdfs:label>
    </owl:Class>
    


    <!-- http://www.semanticweb.org/allalihoussam/ontologies/2025/3/untitled-ontology-11/TransportationMode -->

    <owl:Class rdf:about="http://www.semanticweb.org/allalihoussam/ontologies/2025/3/untitled-ontology-11/TransportationMode">
        <rdfs:comment>“Indicates the travel mode used in a trip segment, such as train, bus, airplane, rideshare, or ferry.”</rdfs:comment>
        <rdfs:label>Transportation Mode</rdfs:label>
    </owl:Class>
    


    <!-- http://www.semanticweb.org/allalihoussam/ontologies/2025/3/untitled-ontology-11/TripPlan -->

    <owl:Class rdf:about="http://www.semanticweb.org/allalihoussam/ontologies/2025/3/untitled-ontology-11/TripPlan">
        <rdfs:subClassOf>
            <owl:Restriction>
                <owl:onProperty rdf:resource="http://www.semanticweb.org/allalihoussam/ontologies/2025/3/untitled-ontology-11/hasItinerary"/>
                <owl:minQualifiedCardinality rdf:datatype="http://www.w3.org/2001/XMLSchema#nonNegativeInteger">1</owl:minQualifiedCardinality>
                <owl:onClass rdf:resource="http://www.semanticweb.org/allalihoussam/ontologies/2025/3/untitled-ontology-11/Itinerary"/>
            </owl:Restriction>
        </rdfs:subClassOf>
        <rdfs:comment>“Encapsulates a complete travel plan, which may comprise one or more itineraries or trip segments. It includes details like departure, arrival, and optional return.”</rdfs:comment>
        <rdfs:label>Trip Plan</rdfs:label>
    </owl:Class>
    


    <!-- http://www.semanticweb.org/allalihoussam/ontologies/2025/3/untitled-ontology-11/TripPlanningService -->

    <owl:Class rdf:about="http://www.semanticweb.org/allalihoussam/ontologies/2025/3/untitled-ontology-11/TripPlanningService">
        <rdfs:comment>“Represents an online platform or service that offers trip planning functionality (e.g., route finders, itinerary generation). It typically supports one or more operations (like searching for itineraries).”</rdfs:comment>
        <rdfs:label>Trip Planning Service</rdfs:label>
    </owl:Class>
    


    <!-- http://www.semanticweb.org/allalihoussam/ontologies/2025/3/untitled-ontology-11/TripSegment -->

    <owl:Class rdf:about="http://www.semanticweb.org/allalihoussam/ontologies/2025/3/untitled-ontology-11/TripSegment">
        <rdfs:subClassOf>
            <owl:Restriction>
                <owl:onProperty rdf:resource="http://www.semanticweb.org/allalihoussam/ontologies/2025/3/untitled-ontology-11/usesTransportationLine"/>
                <owl:qualifiedCardinality rdf:datatype="http://www.w3.org/2001/XMLSchema#nonNegativeInteger">1</owl:qualifiedCardinality>
                <owl:onClass rdf:resource="http://www.semanticweb.org/allalihoussam/ontologies/2025/3/untitled-ontology-11/TransportationLine"/>
            </owl:Restriction>
        </rdfs:subClassOf>
        <rdfs:subClassOf>
            <owl:Restriction>
                <owl:onProperty rdf:resource="http://www.semanticweb.org/allalihoussam/ontologies/2025/3/untitled-ontology-11/duration"/>
                <owl:qualifiedCardinality rdf:datatype="http://www.w3.org/2001/XMLSchema#nonNegativeInteger">1</owl:qualifiedCardinality>
                <owl:onDataRange rdf:resource="http://www.w3.org/2001/XMLSchema#integer"/>
            </owl:Restriction>
        </rdfs:subClassOf>
        <rdfs:comment>“A single continuous portion of travel, typically with a single vehicle (e.g., a single train ride or bus ride). Multiple segments can make up a complete itinerary or trip plan.”</rdfs:comment>
        <rdfs:label>Trip Segment</rdfs:label>
    </owl:Class>
    


    <!-- 
    ///////////////////////////////////////////////////////////////////////////////////////
    //
    // Individuals
    //
    ///////////////////////////////////////////////////////////////////////////////////////
     -->

    


    <!-- http://example.com/instances#OneWayTrip1 -->

    <owl:NamedIndividual rdf:about="http://example.com/instances#OneWayTrip1"/>
    


    <!-- http://example.com/instances#OneWayTrip2 -->

    <owl:NamedIndividual rdf:about="http://example.com/instances#OneWayTrip2"/>
    


    <!-- http://example.com/instances#PlanTripOp -->

    <owl:NamedIndividual rdf:about="http://example.com/instances#PlanTripOp"/>
    


    <!-- http://www.semanticweb.org/allalihoussam/ontologies/2025/3/untitled-ontology-11/BerlinToParis -->

    <owl:NamedIndividual rdf:about="http://www.semanticweb.org/allalihoussam/ontologies/2025/3/untitled-ontology-11/BerlinToParis">
        <rdf:type rdf:resource="http://www.semanticweb.org/allalihoussam/ontologies/2025/3/untitled-ontology-11/OneWayTrip"/>
        <hasMode rdf:resource="http://www.semanticweb.org/allalihoussam/ontologies/2025/3/untitled-ontology-11/ModeTrain"/>
        <hasPricingModel rdf:resource="http://www.semanticweb.org/allalihoussam/ontologies/2025/3/untitled-ontology-11/DynamicPricing2"/>
        <hasStop rdf:resource="http://www.semanticweb.org/allalihoussam/ontologies/2025/3/untitled-ontology-11/StopBerlinHbf"/>
        <hasStop rdf:resource="http://www.semanticweb.org/allalihoussam/ontologies/2025/3/untitled-ontology-11/StopParisEst"/>
        <usesTransportationLine rdf:resource="http://www.semanticweb.org/allalihoussam/ontologies/2025/3/untitled-ontology-11/LineTGVBerlinParis"/>
        <duration rdf:datatype="http://www.w3.org/2001/XMLSchema#integer">360</duration>
        <isInternational rdf:datatype="http://www.w3.org/2001/XMLSchema#boolean">true</isInternational>
        <price rdf:datatype="http://www.w3.org/2001/XMLSchema#decimal">95.50</price>
        <priceCurrency>&quot;EUR&quot;</priceCurrency>
        <remainingSeats rdf:datatype="http://www.w3.org/2001/XMLSchema#integer">40</remainingSeats>
        <rdfs:label>SegmentReturn (Berlin to Paris)</rdfs:label>
    </owl:NamedIndividual>
    


    <!-- http://www.semanticweb.org/allalihoussam/ontologies/2025/3/untitled-ontology-11/BookTicket -->

    <owl:NamedIndividual rdf:about="http://www.semanticweb.org/allalihoussam/ontologies/2025/3/untitled-ontology-11/BookTicket">
        <rdf:type rdf:resource="http://www.semanticweb.org/allalihoussam/ontologies/2025/3/untitled-ontology-11/Operation"/>
    </owl:NamedIndividual>
    


    <!-- http://www.semanticweb.org/allalihoussam/ontologies/2025/3/untitled-ontology-11/CologneConnection -->

    <owl:NamedIndividual rdf:about="http://www.semanticweb.org/allalihoussam/ontologies/2025/3/untitled-ontology-11/CologneConnection">
        <rdf:type rdf:resource="http://www.semanticweb.org/allalihoussam/ontologies/2025/3/untitled-ontology-11/Connection"/>
        <hasMode rdf:resource="http://www.semanticweb.org/allalihoussam/ontologies/2025/3/untitled-ontology-11/ModeTrain"/>
        <transferTime rdf:datatype="http://www.w3.org/2001/XMLSchema#integer">20</transferTime>
        <rdfs:label>Transfer at Cologne Hbf</rdfs:label>
    </owl:NamedIndividual>
    


    <!-- http://www.semanticweb.org/allalihoussam/ontologies/2025/3/untitled-ontology-11/DynamicPricing1 -->

    <owl:NamedIndividual rdf:about="http://www.semanticweb.org/allalihoussam/ontologies/2025/3/untitled-ontology-11/DynamicPricing1">
        <rdf:type rdf:resource="http://www.semanticweb.org/allalihoussam/ontologies/2025/3/untitled-ontology-11/DynamicPricingModel"/>
        <rdfs:comment>&quot;Price fluctuates based on seat availability or demand.&quot;</rdfs:comment>
        <rdfs:label>ICE Dynamic Pricing Model</rdfs:label>
    </owl:NamedIndividual>
    


    <!-- http://www.semanticweb.org/allalihoussam/ontologies/2025/3/untitled-ontology-11/DynamicPricing2 -->

    <owl:NamedIndividual rdf:about="http://www.semanticweb.org/allalihoussam/ontologies/2025/3/untitled-ontology-11/DynamicPricing2">
        <rdf:type rdf:resource="http://www.semanticweb.org/allalihoussam/ontologies/2025/3/untitled-ontology-11/DynamicPricingModel"/>
        <rdfs:comment>&quot;Return trip also uses a dynamic pricing approach.&quot;</rdfs:comment>
        <rdfs:label>Return Trip Dynamic Pricing</rdfs:label>
    </owl:NamedIndividual>
    


    <!-- http://www.semanticweb.org/allalihoussam/ontologies/2025/3/untitled-ontology-11/FixedPricing1 -->

    <owl:NamedIndividual rdf:about="http://www.semanticweb.org/allalihoussam/ontologies/2025/3/untitled-ontology-11/FixedPricing1">
        <rdf:type rdf:resource="http://www.semanticweb.org/allalihoussam/ontologies/2025/3/untitled-ontology-11/FixedPricingModel"/>
        <rdfs:comment>&quot;Price remains constant regardless of seat availability.&quot;</rdfs:comment>
        <rdfs:label>TGV Fixed Pricing Model</rdfs:label>
    </owl:NamedIndividual>
    


    <!-- http://www.semanticweb.org/allalihoussam/ontologies/2025/3/untitled-ontology-11/LineICECologneBerlin -->

    <owl:NamedIndividual rdf:about="http://www.semanticweb.org/allalihoussam/ontologies/2025/3/untitled-ontology-11/LineICECologneBerlin">
        <rdf:type rdf:resource="http://www.semanticweb.org/allalihoussam/ontologies/2025/3/untitled-ontology-11/TransportationLine"/>
        <rdfs:label>ICE from Cologne to Berlin Hbf</rdfs:label>
    </owl:NamedIndividual>
    


    <!-- http://www.semanticweb.org/allalihoussam/ontologies/2025/3/untitled-ontology-11/LineTGVBerlinParis -->

    <owl:NamedIndividual rdf:about="http://www.semanticweb.org/allalihoussam/ontologies/2025/3/untitled-ontology-11/LineTGVBerlinParis">
        <rdf:type rdf:resource="http://www.semanticweb.org/allalihoussam/ontologies/2025/3/untitled-ontology-11/TransportationLine"/>
        <rdfs:label>&quot;TGV from Berlin to Paris Est&quot;</rdfs:label>
    </owl:NamedIndividual>
    


    <!-- http://www.semanticweb.org/allalihoussam/ontologies/2025/3/untitled-ontology-11/LineTGVParisCologne -->

    <owl:NamedIndividual rdf:about="http://www.semanticweb.org/allalihoussam/ontologies/2025/3/untitled-ontology-11/LineTGVParisCologne">
        <rdf:type rdf:resource="http://www.semanticweb.org/allalihoussam/ontologies/2025/3/untitled-ontology-11/TransportationLine"/>
        <rdfs:label>TGV from Paris Est to Cologne</rdfs:label>
    </owl:NamedIndividual>
    


    <!-- http://www.semanticweb.org/allalihoussam/ontologies/2025/3/untitled-ontology-11/ModeTrain -->

    <owl:NamedIndividual rdf:about="http://www.semanticweb.org/allalihoussam/ontologies/2025/3/untitled-ontology-11/ModeTrain">
        <rdf:type rdf:resource="http://www.semanticweb.org/allalihoussam/ontologies/2025/3/untitled-ontology-11/TransportationMode"/>
        <modeName>&quot;Train&quot;</modeName>
        <rdfs:label>Train Mode</rdfs:label>
    </owl:NamedIndividual>
    


    <!-- http://www.semanticweb.org/allalihoussam/ontologies/2025/3/untitled-ontology-11/OneWayTrip1 -->

    <owl:NamedIndividual rdf:about="http://www.semanticweb.org/allalihoussam/ontologies/2025/3/untitled-ontology-11/OneWayTrip1">
        <rdf:type rdf:resource="http://www.semanticweb.org/allalihoussam/ontologies/2025/3/untitled-ontology-11/OneWayTrip"/>
        <hasMode rdf:resource="http://www.semanticweb.org/allalihoussam/ontologies/2025/3/untitled-ontology-11/ModeTrain"/>
        <hasPricingModel rdf:resource="http://www.semanticweb.org/allalihoussam/ontologies/2025/3/untitled-ontology-11/FixedPricing1"/>
        <hasStop rdf:resource="http://www.semanticweb.org/allalihoussam/ontologies/2025/3/untitled-ontology-11/StopCologneHbf"/>
        <hasStop rdf:resource="http://www.semanticweb.org/allalihoussam/ontologies/2025/3/untitled-ontology-11/StopParisEst"/>
        <usesTransportationLine rdf:resource="http://www.semanticweb.org/allalihoussam/ontologies/2025/3/untitled-ontology-11/LineTGVParisCologne"/>
        <duration rdf:datatype="http://www.w3.org/2001/XMLSchema#integer">200</duration>
        <isInternational rdf:datatype="http://www.w3.org/2001/XMLSchema#boolean">true</isInternational>
        <price rdf:datatype="http://www.w3.org/2001/XMLSchema#decimal">60.00</price>
        <priceCurrency>&quot;EUR&quot;</priceCurrency>
        <remainingSeats rdf:datatype="http://www.w3.org/2001/XMLSchema#integer">50</remainingSeats>
        <rdfs:label>Segment Paris to Cologne (TGV)</rdfs:label>
    </owl:NamedIndividual>
    


    <!-- http://www.semanticweb.org/allalihoussam/ontologies/2025/3/untitled-ontology-11/OneWayTrip2 -->

    <owl:NamedIndividual rdf:about="http://www.semanticweb.org/allalihoussam/ontologies/2025/3/untitled-ontology-11/OneWayTrip2">
        <rdf:type rdf:resource="http://www.semanticweb.org/allalihoussam/ontologies/2025/3/untitled-ontology-11/OneWayTrip"/>
        <hasConnection rdf:resource="http://www.semanticweb.org/allalihoussam/ontologies/2025/3/untitled-ontology-11/CologneConnection"/>
        <hasMode rdf:resource="http://www.semanticweb.org/allalihoussam/ontologies/2025/3/untitled-ontology-11/ModeTrain"/>
        <hasPricingModel rdf:resource="http://www.semanticweb.org/allalihoussam/ontologies/2025/3/untitled-ontology-11/DynamicPricing1"/>
        <hasStop rdf:resource="http://www.semanticweb.org/allalihoussam/ontologies/2025/3/untitled-ontology-11/StopBerlinHbf"/>
        <hasStop rdf:resource="http://www.semanticweb.org/allalihoussam/ontologies/2025/3/untitled-ontology-11/StopCologneHbf"/>
        <usesTransportationLine rdf:resource="http://www.semanticweb.org/allalihoussam/ontologies/2025/3/untitled-ontology-11/LineICECologneBerlin"/>
        <duration rdf:datatype="http://www.w3.org/2001/XMLSchema#integer">240</duration>
        <isInternational rdf:datatype="http://www.w3.org/2001/XMLSchema#boolean">false</isInternational>
        <price rdf:datatype="http://www.w3.org/2001/XMLSchema#decimal">79.99</price>
        <priceCurrency>&quot;EUR&quot;</priceCurrency>
        <remainingSeats rdf:datatype="http://www.w3.org/2001/XMLSchema#integer">20</remainingSeats>
        <rdfs:label>Segment Cologne to Berlin (ICE)</rdfs:label>
    </owl:NamedIndividual>
    


    <!-- http://www.semanticweb.org/allalihoussam/ontologies/2025/3/untitled-ontology-11/ParisBerlinRoundTrip -->

    <owl:NamedIndividual rdf:about="http://www.semanticweb.org/allalihoussam/ontologies/2025/3/untitled-ontology-11/ParisBerlinRoundTrip">
        <rdf:type rdf:resource="http://www.semanticweb.org/allalihoussam/ontologies/2025/3/untitled-ontology-11/RoundTripPlan"/>
        <hasItinerary rdf:resource="http://example.com/instances#OneWayTrip1"/>
        <hasItinerary rdf:resource="http://example.com/instances#OneWayTrip2"/>
        <hasReturnTrip rdf:resource="http://www.semanticweb.org/allalihoussam/ontologies/2025/3/untitled-ontology-11/BerlinToParis"/>
        <rdfs:label>&quot;Round Trip Plan: Paris &lt;-&gt; Berlin&quot;</rdfs:label>
    </owl:NamedIndividual>
    


    <!-- http://www.semanticweb.org/allalihoussam/ontologies/2025/3/untitled-ontology-11/PlanTripOp -->

    <owl:NamedIndividual rdf:about="http://www.semanticweb.org/allalihoussam/ontologies/2025/3/untitled-ontology-11/PlanTripOp">
        <rdf:type rdf:resource="http://www.semanticweb.org/allalihoussam/ontologies/2025/3/untitled-ontology-11/PlanTripOperation"/>
        <maxConnectionsAllowed rdf:datatype="http://www.w3.org/2001/XMLSchema#integer">2</maxConnectionsAllowed>
        <rdfs:label>&quot;Plan a MultiLeg Trip&quot;</rdfs:label>
    </owl:NamedIndividual>
    


    <!-- http://www.semanticweb.org/allalihoussam/ontologies/2025/3/untitled-ontology-11/StopBerlinHbf -->

    <owl:NamedIndividual rdf:about="http://www.semanticweb.org/allalihoussam/ontologies/2025/3/untitled-ontology-11/StopBerlinHbf">
        <rdf:type rdf:resource="http://www.semanticweb.org/allalihoussam/ontologies/2025/3/untitled-ontology-11/Stop"/>
        <rdfs:label>Berlin Hauptbahnhof</rdfs:label>
    </owl:NamedIndividual>
    


    <!-- http://www.semanticweb.org/allalihoussam/ontologies/2025/3/untitled-ontology-11/StopCologneHbf -->

    <owl:NamedIndividual rdf:about="http://www.semanticweb.org/allalihoussam/ontologies/2025/3/untitled-ontology-11/StopCologneHbf">
        <rdf:type rdf:resource="http://www.semanticweb.org/allalihoussam/ontologies/2025/3/untitled-ontology-11/Stop"/>
        <rdfs:label>Koln Hauptbahnhof (Cologne Hbf)</rdfs:label>
    </owl:NamedIndividual>
    


    <!-- http://www.semanticweb.org/allalihoussam/ontologies/2025/3/untitled-ontology-11/StopParisEst -->

    <owl:NamedIndividual rdf:about="http://www.semanticweb.org/allalihoussam/ontologies/2025/3/untitled-ontology-11/StopParisEst">
        <rdf:type rdf:resource="http://www.semanticweb.org/allalihoussam/ontologies/2025/3/untitled-ontology-11/Stop"/>
        <rdfs:label>Paris Est (Station)</rdfs:label>
    </owl:NamedIndividual>
    


    <!-- http://www.semanticweb.org/allalihoussam/ontologies/2025/3/untitled-ontology-11/TravelBuddy -->

    <owl:NamedIndividual rdf:about="http://www.semanticweb.org/allalihoussam/ontologies/2025/3/untitled-ontology-11/TravelBuddy">
        <rdf:type rdf:resource="http://www.semanticweb.org/allalihoussam/ontologies/2025/3/untitled-ontology-11/TripPlanningService"/>
        <hasOperation rdf:resource="http://example.com/instances#PlanTripOp"/>
        <hasOperation rdf:resource="http://www.semanticweb.org/allalihoussam/ontologies/2025/3/untitled-ontology-11/BookTicket"/>
        <rdfs:label>&quot;Travel Buddy&quot;</rdfs:label>
    </owl:NamedIndividual>
</rdf:RDF>



<!-- Generated by the OWL API (version 4.5.29.2024-05-13T12:11:03Z) https://github.com/owlcs/owlapi -->

